[sledge sem] Rework emap invariant
Summary:
The LLVM->LLAIR translation keeps a mapping of variables to expressions.
Previously, the invariants related to that mapping were kept in the
state relation, and so the proof needed show that they were preserved
along execution traces. This wasn't obvious as the state changes in
non-SSA ways during evaluation, but the correctness of the mappings is
heavily based on the program being in SSA form. This change separates
out the invariants, and the proof uses the final mapping that the
compiler builds, which contains all of the relevant bindings that might
be needed during execution.

Reviewed By: jberdine

Differential Revision: D20625109

fbshipit-source-id: d4c2dfe19

sledge/semantics/llvmScript.sml
@@ -828,9 +828,17 @@ Definition prog_ok_def:
     ((* All non-entry blocks have a proper header, and entry blocks don't *)
      ∀fname dec.
        alookup p fname = Some dec ⇒
-       (every (\b. fst b = None ⇔ (snd b).h = Entry) dec.blocks)) ∧
+       every (\b. fst b = None ⇔ (snd b).h = Entry) dec.blocks) ∧
+     ((* The blocks in a definition have distinct labels.*)
+      ∀fname dec.
+       alookup p fname = Some dec ⇒
+       all_distinct (map fst dec.blocks)) ∧
      (* There is a main function *)
-     ∃dec. alookup p (Fn "main") = Some dec
+     (∃dec. alookup p (Fn "main") = Some dec) ∧
+     (* No phi instruction assigns the same register twice *)
+     (∀ip from_l phis.
+       get_instr p ip (Inr (from_l, phis)) ⇒
+       all_distinct (map (λp. case p of Phi r _ _ => r) phis))
 End
 
 (* All call frames have a good return address, and the stack allocations of the
